Prove basic TD.Write specs using separation logic

src/SepLogic/Pred/Ptsto.v
@@ -1,7 +1,29 @@
 Require Import Automation.
 
 Require Import SepLogic.Mem.Def.
+Require Import SepLogic.Mem.Upd.
 Require Import SepLogic.Pred.Def.
+
+Definition singleton A V (a:A) (v:V) {AEQ:EqDec A eq} : mem A V :=
+  fun a' => if a == a' then Some v else None.
+
+Lemma ptsto_singleton : forall `(m: mem A V) {AEQ:EqDec A eq} a v,
+    m |= a |-> v ->
+    m = singleton a v.
+Proof.
+  unfold singleton; simpl; intros.
+  extensionality a'.
+  is_eq a a'; intuition.
+Qed.
+
+Lemma ptsto_singleton' : forall A V {AEQ:EqDec A eq} (a:A) (v:V),
+    singleton a v |= a |-> v.
+Proof.
+  unfold singleton; simpl; intros.
+  subst.
+  destruct matches; intuition.
+  destruct matches; intuition.
+Qed.
 
 Theorem ptsto_valid : forall `(m: mem A V) F a v,
     m |= F * a |-> v ->
@@ -11,4 +33,35 @@ Proof.
   apply star_comm in H.
   simpl in *; repeat deex.
   unfold mem_union; simpl_match; auto.
+Qed.
+
+Lemma mem_disjoint_singleton : forall `(m:mem A V) {AEQ:EqDec A eq} a v0 v,
+    mem_disjoint (singleton a v0) m ->
+    mem_disjoint (singleton a v) m.
+Proof.
+  unfold mem_disjoint, singleton; intuition.
+  eapply H; eauto.
+  destruct matches in *; eauto.
+Qed.
+
+Hint Resolve ptsto_singleton'.
+Hint Resolve mem_disjoint_singleton.
+
+Theorem ptsto_upd : forall `(m:mem A V) {AEQ:EqDec A eq} F a v0 v,
+    m |= F * a |-> v0 ->
+    upd m a v |= F * a |-> v.
+Proof.
+  intros.
+  apply star_comm in H.
+  apply star_comm.
+  cbn [pred_prop star] in *; repeat deex.
+  (* TODO: can we get AEQ to be inferred from the context rather than this
+  unshelve t; eauto? *)
+  unshelve eapply ptsto_singleton in H; eauto; subst.
+  exists (singleton a v), m2; intuition eauto.
+  extensionality a'.
+  unfold singleton, mem_union.
+  is_eq a a'; autorewrite with upd; eauto.
+  is_eq a a'; autorewrite with upd; eauto.
+  congruence.
 Qed.
