src/Shallow/TwoDiskProg.v
@@ -12,7 +12,6 @@ Arguments Failed {T}.
 
 Module TD.
 
-
   Inductive Op : Type -> Type :=
   | Read (i:diskId) (a:addr) : Op (DiskResult block)
   | Write (i:diskId) (a:addr) (b:block) : Op (DiskResult unit).
@@ -34,20 +33,34 @@ Module TD.
     | d1 => disk1 state
     end.
 
+  Local Lemma d0_is_some (d_0: disk) (d_1: option disk) :
+    Some d_0 = None -> d_1 = None -> False.
+  Proof.
+    congruence.
+  Qed.
+
+  Local Lemma d1_is_some (d_0: option disk) (d_1: disk) :
+    d_0 = None -> Some d_1 = None -> False.
+  Proof.
+    congruence.
+  Qed.
+
+  Local Notation proof := (ltac:(first [ apply d0_is_some | apply d1_is_some ])) (only parsing).
+
   Definition set_disk (i:diskId) (state:State) (d:disk) : State :=
     match i with
-    | d0 => let 'Disks _ d_1 _ := state in Disks (Some d) d_1 ltac:(congruence)
-    | d1 => let 'Disks d_0 _ _ := state in Disks d_0 (Some d) ltac:(congruence)
+    | d0 => Disks (Some d) (TD.disk1 state) proof
+    | d1 => Disks (TD.disk0 state) (Some d) proof
     end.
 
   Inductive bg_step : State -> State -> Prop :=
   | step_id : forall state, bg_step state state
   | step_fail0 : forall d_0 d_1 pf,
       bg_step (Disks (Some d_0) (Some d_1) pf)
-              (Disks None (Some d_1) ltac:(congruence))
+              (Disks None (Some d_1) proof)
   | step_fail1 : forall d_0 d_1 pf,
       bg_step (Disks (Some d_0) (Some d_1) pf)
-              (Disks (Some d_0) None ltac:(congruence)).
+              (Disks (Some d_0) None proof).
 
   Inductive op_step : Semantics Op State :=
   | step_read : forall a i r state,
