src/Shallow/TwoDiskProgTheorems.v
@@ -22,7 +22,32 @@ Proof.
   destruct md; intuition.
 Qed.
 
-Hint Resolve md_pred_weaken.
+Theorem md_pred_none : forall md F (P:Prop),
+    P ->
+    md = None ->
+    md_pred md F P.
+Proof.
+  intros; subst; intuition.
+Qed.
+
+Hint Resolve md_pred_weaken md_pred_none.
+
+Ltac start_spec :=
+  unfold prog_spec; intros;
+    repeat match goal with
+           | [ H: context[let '(a, b) := ?p in _] |- _ ] =>
+             let a := fresh a in
+             let b := fresh b in
+             destruct p as [a b]
+           end;
+    simpl in *;
+    safe_intuition;
+    try match goal with
+        | [ H: exec _ (Prim _) _ _ |- _ ] =>
+          eapply (inversion_prim_exec H); intros
+        end;
+    repeat deex;
+    try solve [ intuition eauto ].
 
 Theorem Read0_ok : forall a,
     prog_spec
@@ -47,30 +72,21 @@ Theorem Read0_ok : forall a,
       (Prim (TD.Read d0 a))
       TD.step.
 Proof.
-  unfold prog_spec; intros;
-    repeat match goal with
-           | [ H: context[let '(a, b) := ?p in _] |- _ ] =>
-             let a := fresh a in
-             let b := fresh b in
-             destruct p as [a b]
-           end;
-    simpl in *;
-    safe_intuition.
-  eapply (inversion_prim_exec H0); intros; eauto.
-  TD.inv_step.
-  inversion H2; subst; clear H2; simpl in *; repeat simpl_match; eauto.
-  destruct (TD.disk0 state') eqn:?; simpl in *; subst.
-  pose proof (ptsto_valid H).
-  unfold disk_get in *.
-  simpl_match; subst; intuition eauto.
-  destruct state'; simpl in *; subst; intuition eauto.
-  destruct disk1; simpl; intuition eauto.
-  pose proof (ptsto_valid H).
-  unfold disk_get in *.
-  simpl_match; subst; intuition eauto.
-  destruct v; subst; intuition eauto.
-  destruct (TD.disk0 state'); simpl in *; eauto.
-  apply lift_extract in H4; contradiction.
+  start_spec.
+  - TD.inv_step.
+    inversion H2; subst; clear H2; simpl in *; repeat simpl_match; eauto.
+    destruct (TD.disk0 state') eqn:?; simpl in *; subst.
+    pose proof (ptsto_valid H).
+    unfold disk_get in *.
+    simpl_match; subst; intuition eauto.
+    destruct state'; simpl in *; subst; intuition eauto.
+    destruct disk1; simpl; intuition eauto.
+    pose proof (ptsto_valid H).
+    unfold disk_get in *.
+    simpl_match; subst; intuition eauto.
+  - destruct v; subst; intuition eauto.
+    destruct (TD.disk0 state'); simpl in *; eauto.
+    apply lift_extract in H4; contradiction.
 Qed.
 
 Theorem Read1_ok : forall a,
@@ -96,28 +112,89 @@ Theorem Read1_ok : forall a,
       (Prim (TD.Read d1 a))
       TD.step.
 Proof.
-  unfold prog_spec; intros;
-    repeat match goal with
-           | [ H: context[let '(a, b) := ?p in _] |- _ ] =>
-             let a := fresh a in
-             let b := fresh b in
-             destruct p as [a b]
-           end;
-    simpl in *;
-    safe_intuition.
-  eapply (inversion_prim_exec H0); intros; eauto.
-  TD.inv_step.
-  inversion H2; subst; clear H2; simpl in *; repeat simpl_match; eauto.
-  destruct (TD.disk1 state') eqn:?; simpl in *; subst.
-  pose proof (ptsto_valid H1).
-  unfold disk_get in *.
-  simpl_match; subst; intuition eauto.
-  destruct state'; simpl in *; subst; intuition eauto.
-  destruct disk0; simpl; intuition eauto.
-  pose proof (ptsto_valid H1).
-  unfold disk_get in *.
-  simpl_match; subst; intuition eauto.
-  destruct v; subst; intuition eauto.
-  destruct (TD.disk1 state'); simpl in *; eauto.
-  apply lift_extract in H5; contradiction.
+  start_spec.
+  - TD.inv_step.
+    inversion H2; subst; clear H2; simpl in *; repeat simpl_match; eauto.
+    destruct (TD.disk1 state') eqn:?; simpl in *; subst.
+    pose proof (ptsto_valid H1).
+    unfold disk_get in *.
+    simpl_match; subst; intuition eauto.
+    destruct state'; simpl in *; subst; intuition eauto.
+    destruct disk0; simpl; intuition eauto.
+    pose proof (ptsto_valid H1).
+    unfold disk_get in *.
+    simpl_match; subst; intuition eauto.
+  - destruct v; subst; intuition eauto.
+    destruct (TD.disk1 state'); simpl in *; eauto.
+    apply lift_extract in H5; contradiction.
+Qed.
+
+Hint Resolve ptsto_diskUpd.
+
+Theorem Write0_ok : forall a b,
+    prog_spec
+      (fun '(F0, F1, v0) state =>
+         {|
+           pre := md_pred (TD.disk0 state) (F0 * a |-> v0)%pred True /\
+                  md_pred (TD.disk1 state) F1 True;
+           post :=
+             fun r state' =>
+               match r with
+               | Working _ => md_pred (TD.disk0 state') (F0 * a |-> b)%pred False /\
+                             md_pred (TD.disk1 state') F1 True
+               | Failed => md_pred (TD.disk0 state') (lift False) True /\
+                          md_pred (TD.disk1 state') F1 False
+               end;
+           crash :=
+             fun state' =>
+               (md_pred (TD.disk0 state') (F0 * a |-> v0)%pred True \/
+                md_pred (TD.disk0 state') (F0 * a |-> b)%pred True) /\
+               md_pred (TD.disk1 state') F1 True;
+         |})
+      (Prim (TD.Write d0 a b))
+      TD.step.
+Proof.
+  start_spec.
+  - TD.inv_step; repeat subst_var; simpl.
+    inversion H2; subst; clear H2; simpl in *; eauto.
+    destruct matches; simpl in *; intuition eauto.
+    destruct (TD.disk1 x) eqn:?; simpl; eauto.
+    destruct x; eauto.
+  - destruct v; intuition eauto.
+    destruct (TD.disk0 state'); simpl in *; eauto.
+    apply lift_extract in H4; contradiction.
+Qed.
+
+Theorem Write1_ok : forall a b,
+    prog_spec
+      (fun '(F0, F1, v0) state =>
+         {|
+           pre := md_pred (TD.disk0 state) F0 True /\
+                  md_pred (TD.disk1 state) (F1 * a |-> v0)%pred True;
+           post :=
+             fun r state' =>
+               match r with
+               | Working _ => md_pred (TD.disk0 state') F0 True /\
+                             md_pred (TD.disk1 state') (F1 * a |-> b)%pred False
+               | Failed => md_pred (TD.disk0 state') F0 False /\
+                          md_pred (TD.disk1 state') (lift False) True
+               end;
+           crash :=
+             fun state' =>
+               md_pred (TD.disk0 state') F0 True /\
+               (md_pred (TD.disk1 state') (F1 * a |-> v0)%pred True \/
+                md_pred (TD.disk1 state') (F1 * a |-> b)%pred True);
+         |})
+      (Prim (TD.Write d1 a b))
+      TD.step.
+Proof.
+  start_spec.
+  - TD.inv_step; repeat subst_var; simpl.
+    inversion H2; subst; clear H2; simpl in *; eauto.
+    destruct matches; simpl in *; intuition eauto.
+    destruct (TD.disk0 x) eqn:?; simpl; eauto.
+    destruct x; eauto.
+  - destruct v; intuition eauto.
+    destruct (TD.disk1 state'); simpl in *; eauto.
+    apply lift_extract in H5; contradiction.
 Qed.
